Add a sequencing construct to XmlLang

platform/XmlLang.v
@@ -21,10 +21,45 @@ Inductive pat :=
 (* Match one pattern and then another in the part of the XML tree right after the match of the first. *)
 | Ordered (p1 p2 : pat).
 
-(* A full program: find all matches of a pattern, outputting the value of a variable for each. *)
+(* Language for generating XML code *)
+Inductive xml :=
+| XCdata (const : string)
+| XVar (text : string)
+| XTag (tag : string) (inner : list xml).
+
+Section xml_ind'.
+  Variable P : xml -> Prop.
+
+  Hypothesis H_Cdata : forall const, P (XCdata const).
+
+  Hypothesis H_Var : forall text, P (XVar text).
+
+  Hypothesis H_Tag : forall tag inner, List.Forall P inner -> P (XTag tag inner).
+
+  Fixpoint xml_ind' (xm : xml) : P xm :=
+    match xm with
+      | XCdata const => H_Cdata const
+      | XVar text => H_Var text
+      | XTag tag inner => H_Tag tag ((fix xmls_ind (xms : list xml) : List.Forall P xms :=
+        match xms with
+          | nil => Forall_nil _
+          | xm :: xms' => Forall_cons _ (xml_ind' xm) (xmls_ind xms')
+        end) inner)
+    end.
+End xml_ind'.
+
+Opaque xml_ind'.
+
+
+(* Language of actions to take for matched patterns *)
+Inductive action :=
+| Output (xm : xml)
+| Seq (a1 a2 : action).
+
+(* A full program: find all matches of a pattern, running an action for each. *)
 Record program := {
   Pattern : pat;
-  Output : xml
+  Action : action
 }.
 
 
@@ -39,13 +74,13 @@ Fixpoint freeVar (p : pat) (x : string) : Prop :=
     | Ordered p1 p2 => freeVar p1 x \/ freeVar p2 x
   end.
 
-Fixpoint wfPat (p : pat) : Prop :=
+Fixpoint pwf (p : pat) : Prop :=
   match p with
     | Cdata const => goodSize (String.length const)
     | Var _ => True
-    | Tag tag inner => goodSize (String.length tag) /\ wfPat inner
-    | Both p1 p2 => wfPat p1 /\ wfPat p2 /\ (forall x, freeVar p1 x -> ~freeVar p2 x)
-    | Ordered p1 p2 => wfPat p1 /\ wfPat p2 /\ (forall x, freeVar p1 x -> ~freeVar p2 x)
+    | Tag tag inner => goodSize (String.length tag) /\ pwf inner
+    | Both p1 p2 => pwf p1 /\ pwf p2 /\ (forall x, freeVar p1 x -> ~freeVar p2 x)
+    | Ordered p1 p2 => pwf p1 /\ pwf p2 /\ (forall x, freeVar p1 x -> ~freeVar p2 x)
   end%type.
 
 Fixpoint allCdatas (p : pat) : list string :=
@@ -58,7 +93,24 @@ Fixpoint allCdatas (p : pat) : list string :=
   end.
 
 
-(** * Compiling patterns *)
+(** * Our versions of the auxiliary functions from XmlOutput *)
+
+Fixpoint xwf (xm : xml) : Prop :=
+  match xm with
+    | XCdata const => goodSize (String.length const)
+    | XVar _ => True
+    | XTag tag inner => goodSize (String.length tag + 3) /\ ForallR xwf inner
+  end.
+
+Fixpoint xfreeVar (xm : xml) (x : string) : Prop :=
+  match xm with
+    | XCdata _ => False
+    | XVar text => x = text
+    | XTag _ inner => ExistsR (fun xm' => xfreeVar xm' x) inner
+  end.
+
+
+(** * Compiling to other [Xml*] modules' languages *)
 
 Fixpoint compilePat (p : pat) : XmlSearch.pat :=
   match p with
@@ -67,15 +119,35 @@ Fixpoint compilePat (p : pat) : XmlSearch.pat :=
     | Tag tag inner => XmlSearch.Tag tag (compilePat inner)
     | Both p1 p2 => XmlSearch.Both (compilePat p1) (compilePat p2)
     | Ordered p1 p2 => XmlSearch.Ordered (compilePat p1) (compilePat p2)
-  end%string.
+  end.
+
+Fixpoint compileXml (p : xml) : XmlOutput.xml :=
+  match p with
+    | XCdata const => XmlOutput.Cdata const
+    | XVar text => XmlOutput.Var (text ++ "_start") (text ++ "_len")
+    | XTag tag inner => XmlOutput.Tag tag (map compileXml inner)
+  end.
+
+
+(** * Combined well-formedness and related lemmas *)
+
+Fixpoint awf (a : action) : Prop :=
+  match a with
+    | Output xm => xwf xm
+    | Seq a1 a2 => awf a1 /\ awf a2
+  end.
+
+Fixpoint afreeVar (a : action) (x : string) : Prop :=
+  match a with
+    | Output xm => xfreeVar xm x
+    | Seq a1 a2 => afreeVar a1 x \/ afreeVar a2 x
+  end.
 
 Definition wf (pr : program) :=
-  wfPat (Pattern pr)
-  /\ XmlOutput.wf (Output pr)
-  /\ cdatasGood (XmlSearch.allCdatas (compilePat (Pattern pr)))
-  /\ forall start len, XmlOutput.freeVar (Output pr) (start, len)
-    -> exists x, start = (x ++ "_start")%string /\ len = (x ++ "_len")%string
-      /\ freeVar (Pattern pr) x.
+  pwf (Pattern pr)
+  /\ awf (Action pr)
+  /\ forall x, afreeVar (Action pr) x
+    -> freeVar (Pattern pr) x.
 
 Fixpoint allCdatas_both (p : pat) : list string :=
   match p with
@@ -238,7 +310,7 @@ Qed.
 Local Hint Resolve allCdatas_freeVar.
 
 Lemma wf_compile : forall p,
-  wfPat p
+  pwf p
   -> XmlSearch.wf (compilePat p).
   induction p; simpl; intuition;
     repeat match goal with
@@ -249,7 +321,7 @@ Qed.
 Local Hint Immediate wf_compile.
 
 Lemma wf_NoDup : forall p,
-  wfPat p
+  pwf p
   -> NoDup (allCdatas p).
   induction p; simpl; intuition; try NoDup; eauto using NoDup_app.
 Qed.
@@ -258,49 +330,6 @@ Qed.
 (** * Compiling programs *)
 
 Section compileProgram.
-  (** First, create a [vcgen] version that knows about [Pat], with some shameless copy-and-paste. *)
-
-  Ltac vcgen_simp := cbv beta iota zeta delta [WrapC Wrap Pat Out
-    map app imps
-    LabelMap.add Entry Blocks Postcondition VerifCond
-    Straightline_ Seq_ Diverge_ Fail_ Skip_ Assert_
-    Structured.If_ Structured.While_ Goto_ Structured.Call_ IGoto
-    setArgs Programming.Reserved Programming.Formals Programming.Precondition
-    importsMap fullImports buildLocals blocks union Nplus Nsucc length N_of_nat
-    List.fold_left ascii_lt string_lt label'_lt
-    LabelKey.compare' LabelKey.compare LabelKey.eq_dec
-    LabelMap.find
-    toCmd Seq Instr Diverge Fail Skip Assert_
-    Programming.If_ Programming.While_ Goto Programming.Call_ RvImm'
-    Assign' localsInvariant localsInvariantCont
-    regInL lvalIn immInR labelIn variableSlot string_eq ascii_eq
-    andb Bool.eqb qspecOut
-    ICall_ Structured.ICall_
-    Assert_ Structured.Assert_
-    LabelMap.Raw.find LabelMap.this LabelMap.Raw.add
-    LabelMap.empty LabelMap.Raw.empty string_dec
-    Ascii.ascii_dec string_rec string_rect sumbool_rec sumbool_rect Ascii.ascii_rec Ascii.ascii_rect
-    Bool.bool_dec bool_rec bool_rect eq_rec_r eq_rec eq_rect eq_sym
-    fst snd labl
-    Ascii.N_of_ascii Ascii.N_of_digits N.compare Nmult Pos.compare Pos.compare_cont
-    Pos.mul Pos.add LabelMap.Raw.bal
-    Int.Z_as_Int.gt_le_dec Int.Z_as_Int.ge_lt_dec LabelMap.Raw.create
-    ZArith_dec.Z_gt_le_dec Int.Z_as_Int.plus Int.Z_as_Int.max LabelMap.Raw.height
-    ZArith_dec.Z_gt_dec Int.Z_as_Int._1 BinInt.Z.add Int.Z_as_Int._0 Int.Z_as_Int._2 BinInt.Z.max
-    ZArith_dec.Zcompare_rec ZArith_dec.Z_ge_lt_dec BinInt.Z.compare ZArith_dec.Zcompare_rect
-    ZArith_dec.Z_ge_dec label'_eq label'_rec label'_rect
-    COperand1 CTest COperand2 Pos.succ
-    makeVcs
-    Note_ Note__
-    IGotoStar_ IGotoStar AssertStar_ AssertStar
-    Cond_ Cond
-  ].
-
-  Ltac vcgen := structured_auto vcgen_simp.
-
-
-  (** Now, on to the interesting part.... *)
-
   Variable pr : program.
 
   Definition numCdatas := length (allCdatas_both (Pattern pr)).
@@ -316,73 +345,6 @@ Section compileProgram.
       * [| length bsI = wordToNat (V "len") |] * [| length bsO = wordToNat (V "olen") |]
     POST[R] Ex bsO', array8 bsI (V "buf") * array8 bsO' (V "obuf") * mallocHeap 0
       * [| length bsO' = length bsO |] * [| R <= V "olen" |].
-
-  Definition m := bimport [["xml_lex"!"next" @ [nextS], "xml_lex"!"position" @ [positionS],
-                            "xml_lex"!"setPosition" @ [setPositionS], "xml_lex"!"tokenStart" @ [tokenStartS],
-                            "xml_lex"!"tokenLength" @ [tokenLengthS], "malloc"!"malloc" @ [mallocS],
-                            "malloc"!"free" @ [freeS], "sys"!"abort" @ [abortS], "sys"!"printInt" @ [printIntS],
-                            "xml_lex"!"init" @ [initS], "xml_lex"!"delete" @ [deleteS],
-                            "array8"!"copy" @ [copyS] ]]
-
-    bmodule "xml_prog" {{
-      {|
-        FName := "main";
-        FVars := lvars;
-        FReserved := 11;
-        FPrecondition := Precondition mainS None;
-        FBody := Seq (Assign' ((fun _ => LvMem (Indir Sp O)):lvalue') Rp)
-        (Seq (fun _ _ =>
-          Structured nil
-          (fun im mn _ =>
-            Structured.Assert_ im mn
-            (Precondition mainS (Some lvars))))
-        ("lex" <-- Call "xml_lex"!"init"("len")
-         [Al bsI, Al bsO,
-           PRE[V, R] array8 bsI (V "buf") * array8 bsO (V "obuf") * mallocHeap 0 * xmlp (V "len") R
-             * [| length bsI = wordToNat (V "len") |] * [| length bsO = wordToNat (V "olen") |]
-           POST[R'] Ex bsO', array8 bsI (V "buf") * array8 bsO' (V "obuf") * mallocHeap 0
-             * [| length bsO' = length bsO |] * [| R' <= V "olen" |]%word ];;
-         "stack" <- 0;;
-         "opos" <- 0;;
-         "overflowed" <- 0;;
-
-         Pat (fun bsO V => array8 bsO (V "obuf") * [| length bsO = wordToNat (V "olen") |]
-           * [| V "opos" <= V "olen" |]%word)%Sep
-         (fun bsO V R => Ex bsO', array8 bsO' (V "obuf") * [| length bsO' = length bsO |]
-           * [| R <= V "olen" |]%word)%Sep
-         (compilePat (Pattern pr))
-         (Out
-           (fun (_ : unit) V => mallocHeap 0 * xmlp (V "len") (V "lex")
-             * Ex ls, sll ls (V "stack") * [| stackOk ls (V "len") |])%Sep
-           (fun _ V R => [| R <= V "olen" |]%word * mallocHeap 0)%Sep
-           (XmlSearch.allCdatas (compilePat (Pattern pr)))
-           (Output pr));;
-
-         Call "xml_lex"!"delete"("lex")
-         [Al ls,
-           PRE[V] [| V "opos" <= V "olen" |]%word * mallocHeap 0 * sll ls (V "stack")
-           POST[R] [| R <= V "olen" |]%word * mallocHeap 0];;
-
-         [Al ls,
-           PRE[V] [| V "opos" <= V "olen" |]%word * mallocHeap 0 * sll ls (V "stack")
-           POST[R] [| R <= V "olen" |]%word * mallocHeap 0]
-         While ("stack" <> 0) {
-           "lex" <- "stack";;
-           "stack" <-* "stack"+4;;
-
-           Call "malloc"!"free"(0, "lex", 2)
-           [Al ls,
-             PRE[V] [| V "opos" <= V "olen" |]%word * mallocHeap 0 * sll ls (V "stack")
-             POST[R] [| R <= V "olen" |]%word * mallocHeap 0]
-         };;
-
-         If ("overflowed" = 1) {
-           Return 0
-         } else {
-           Return "opos"
-         }))%SP
-      |}
-    }}.
 
   Hypothesis wellFormed : wf pr.
 
@@ -471,7 +433,15 @@ Section compileProgram.
         end;
     descend; reger; try rewrite inBounds_sel in *.
 
-  Ltac my_evaluate := evaluate SinglyLinkedList.hints.
+  Ltac clear_fancier :=
+    try match goal with
+          | [ H : importsGlobal _ |- _ ] => clear dependent H
+        end;
+    repeat match goal with
+             | [ H : LabelMap.find _ _ = _ |- _ ] => clear H
+           end.
+
+  Ltac my_evaluate := clear_fancier; evaluate SinglyLinkedList.hints.
   Ltac my_step := step SinglyLinkedList.hints.
 
   Ltac invoke1 :=
@@ -481,12 +451,33 @@ Section compileProgram.
 
   Ltac t' := post; repeat invoke1; prep; my_evaluate; my_descend; repeat (my_step; my_descend); eauto.
 
+  Lemma freeVar_compile' : forall x p,
+    freeVar p x
+    -> In (x ++ "_start", x ++ "_len")%string (XmlSearch.allCdatas (compilePat p)).
+    induction p; simpl; intuition.
+  Qed.
+
+  Lemma freeVar_start : forall x p,
+    freeVar p x
+    -> In (x ++ "_start")%string (allCdatas_both p).
+    induction p; simpl; intuition.
+  Qed.
+
+  Lemma freeVar_len : forall x p,
+    freeVar p x
+    -> In (x ++ "_len")%string (allCdatas_both p).
+    induction p; simpl; intuition.
+  Qed.
+
+  Hint Immediate freeVar_start freeVar_len.
+
   Ltac easy :=
     try match goal with
           | [ H : XmlOutput.freeVar _ _, H' : forall start len : string, _ |- _ ] =>
             apply H' in H; post; subst
         end;
-    solve [ hnf; simpl; intuition (subst; try congruence; eauto) ].
+    solve [ hnf; simpl; intuition (subst; try congruence;
+      eauto using freeVar_compile', freeVar_start, freeVar_len) ].
 
   Ltac pre := try destruct wellFormed;
     repeat match goal with
@@ -518,7 +509,7 @@ Section compileProgram.
 
   Hint Immediate inBounds_swizzle.
 
-  Ltac prove_irrel :=
+  Ltac prove_irrel := clear_fancier;
     repeat match goal with
              | [ V : vals |- _ ] =>
                match goal with
@@ -544,30 +535,10 @@ Section compileProgram.
     induction p; simpl; intuition.
   Qed.
 
-  Lemma freeVar_compile' : forall x p,
-    freeVar p x
-    -> In (x ++ "_start", x ++ "_len")%string (XmlSearch.allCdatas (compilePat p)).
-    induction p; simpl; intuition.
-  Qed.
-
   Hint Extern 1 (_ <= _)%nat =>
     match goal with
       | [ H : inBounds _ _ |- _ ] => eapply Forall_forall in H; [ | eauto using freeVar_compile' ]
     end.
-
-  Lemma freeVar_start : forall x p,
-    freeVar p x
-    -> In (x ++ "_start")%string (allCdatas_both p).
-    induction p; simpl; intuition.
-  Qed.
-
-  Lemma freeVar_len : forall x p,
-    freeVar p x
-    -> In (x ++ "_len")%string (allCdatas_both p).
-    induction p; simpl; intuition.
-  Qed.
-
-  Hint Immediate freeVar_start freeVar_len.
 
   Hint Extern 1 (NoDup (_ :: _)) => repeat constructor; simpl; intuition injy.
 
@@ -577,11 +548,350 @@ Section compileProgram.
   Hint Constructors unit.
   Hint Immediate freeVar_compile'.
 
+  Lemma Forall_map : forall A B (f : A -> B) (P : B -> Prop) ls,
+    List.Forall (fun x => P (f x)) ls
+    -> List.Forall P (map f ls).
+    induction 1; simpl; auto.
+  Qed.
+
+  Lemma output_wf : forall xm,
+    xwf xm
+    -> XmlOutput.wf (compileXml xm).
+    induction xm using xml_ind'; simpl; intuition.
+    apply Forall_ForallR; apply Forall_map; eapply Forall_impl2; [
+      eassumption
+      | apply ForallR_Forall; eassumption
+      | auto ].
+  Qed.
+
+  Hint Immediate output_wf.
+
+
+  (** ** Action compilation *)
+
+  Section compileAction.
+    Variable p : pat.
+
+    Definition SimpleSeq (ch1 ch2 : chunk) : chunk := fun ns res =>
+      Structured nil (fun im mn H => Seq_ H (toCmd ch1 mn H ns res) (toCmd ch2 mn H ns res)).
+
+    Infix ";;" := SimpleSeq : SP_scope.
+
+    Fixpoint compileAction' (a : action) : chunk :=
+      match a with
+        | Output xm => 
+          Out
+          (fun (_ : unit) V => mallocHeap 0 * xmlp (V "len") (V "lex")
+            * Ex ls, sll ls (V "stack") * [| stackOk ls (V "len") |])%Sep
+          (fun _ V R => [| R <= V "olen" |]%word * mallocHeap 0)%Sep
+          (XmlSearch.allCdatas (compilePat p))
+          (compileXml xm)
+        | Seq a1 a2 =>
+          compileAction' a1;;
+          compileAction' a2
+      end%SP.
+
+    Definition ainv :=
+      XmlSearch.inv (fun bsO V => array8 bsO (V "obuf") * [| length bsO = wordToNat (V "olen") |]
+        * [| V "opos" <= V "olen" |]%word)%Sep
+      (fun bsO V R => Ex bsO', array8 bsO' (V "obuf") * [| length bsO' = length bsO |]
+        * [| R <= V "olen" |]%word)%Sep
+      (XmlSearch.allCdatas (compilePat p)).
+
+    Lemma compileAction_post : forall im mn (H : importsGlobal im) ns res a pre,
+      (forall specs st,
+        interp specs (pre st)
+        -> interp specs (ainv true (fun x : W => x) ns res st))
+      -> forall specs st, interp specs (Postcondition (toCmd (compileAction' a) mn H ns res pre) st)
+        -> interp specs (ainv true (fun x : W => x) ns res st).
+      induction a; abstract t.
+    Qed.
+
+    Lemma Exists_map : forall A B (f : A -> B) (P : B -> Prop) ls,
+      List.Exists P (map f ls)
+      -> List.Exists (fun x => P (f x)) ls.
+      induction ls; inversion 1; subst; auto.
+    Qed.
+
+    Lemma Forall_Exists : forall A (P Q : A -> Prop) ls,
+      List.Forall P ls
+      -> List.Exists Q ls
+      -> exists x, P x /\ Q x /\ In x ls.
+      induction 1; inversion 1; subst; simpl; intuition eauto;
+        match goal with
+          | [ H : Logic.ex _ |- _ ] => destruct H; intuition eauto
+        end.
+    Qed.
+
+    Lemma In_ExistsR : forall A (P : A -> Prop) x ls,
+      In x ls
+      -> P x
+      -> ExistsR P ls.
+      induction ls; simpl; intuition.
+    Qed.
+
+    Hint Immediate In_ExistsR.
+
+    Lemma compileXml_freeVar : forall start len xm,
+      XmlOutput.freeVar (compileXml xm) (start, len)
+      -> exists text, xfreeVar xm text
+        /\ start = (text ++ "_start")%string
+        /\ len = (text ++ "_len")%string.
+      induction xm using xml_ind'; simpl; intuition;
+        try match goal with
+              | [ H : (_, _) = (_, _) |- _ ] => injection H; clear H; intros; subst
+            end; eauto.
+      apply ExistsR_Exists in H0; apply Exists_map in H0.
+      eapply Forall_Exists in H; eauto.
+      destruct H; intuition; match goal with
+                               | [ H : Logic.ex _ |- _ ] => destruct H; intuition eauto
+                             end.
+    Qed.
+
+    Lemma underscore_discrim : forall s1 s2,
+      s1 = s2
+      -> ~underscore_free s1
+      -> underscore_free s2
+      -> False.
+      intros; congruence.
+    Qed.
+
+    Lemma compilePat_cdatas : forall p0,
+      cdatasGood (XmlSearch.allCdatas (compilePat p0)).
+      unfold cdatasGood; induction p0; simpl; intuition.
+      constructor; auto; simpl; intuition (eapply underscore_discrim; eauto).
+    Qed.
+
+    Hint Immediate compilePat_cdatas.
+
+    Notation baseVars := ("buf" :: "len" :: "lex" :: "res"
+      :: "tagStart" :: "tagLen" :: "matched" :: "stack" :: "level" :: nil).
+
+    Notation "l ~~ im ~~> s" := (LabelMap.find l%SP im = Some (Precondition s None)) (at level 0).
+
+    Lemma compileAction_vcs : forall im mn (H : importsGlobal im) ns res,
+      ~In "rp" ns
+      -> In "obuf" ns
+      -> In "olen" ns
+      -> In "opos" ns
+      -> In "overflowed" ns
+      -> In "tmp" ns
+      -> In "buf" ns
+      -> incl baseVars ns
+      -> (res >= 7)%nat
+      -> "array8"!"copy" ~~ im ~~> copyS
+      -> forall a pre,
+        (forall specs st,
+          interp specs (pre st)
+          -> interp specs (ainv true (fun x : W => x) ns res st))
+        -> awf a
+        -> (forall text, afreeVar a text -> In (text ++ "_start", text ++ "_len")%string
+          (XmlSearch.allCdatas (compilePat p)))
+        -> (forall text, afreeVar a text -> In (text ++ "_start") ns /\ In (text ++ "_len") ns)%string
+        -> vcs (VerifCond (toCmd (compileAction' a) mn H ns res pre)).
+      induction a; (wrap0;
+        match goal with
+          | [ H : _ |- _ ] =>
+            apply compileXml_freeVar in H; post; subst; solve [
+              eauto | eapply proj1; eauto | eapply proj2; eauto ]
+          | _ => solve [ t ]
+          | _ => repeat (post; intuition idtac;
+            match goal with
+              | [ H : _ |- _ ] => apply H; auto
+            end; try (apply compileAction_post; auto))
+        end).
+    Qed.
+
+    Hint Resolve compileAction_post compileAction_vcs.
+
+    Notation CompileVcs a := (fun im ns res =>
+      (~In "rp" ns) :: In "obuf" ns :: In "olen" ns :: In "opos" ns :: In "overflowed" ns
+      :: In "tmp" ns :: In "buf" ns :: incl baseVars ns
+      :: (res >= 7)%nat
+      :: "array8"!"copy" ~~ im ~~> copyS
+      :: awf a
+      :: (forall text, afreeVar a text -> In (text ++ "_start", text ++ "_len")%string
+        (XmlSearch.allCdatas (compilePat p)))
+      :: (forall text, afreeVar a text -> (In (text ++ "_start") ns /\ In (text ++ "_len") ns)%string)
+      :: nil).
+
+    Definition compileAction (a : action) : chunk.
+      refine (WrapC (compileAction' a)
+        ainv
+        ainv
+        (CompileVcs a) _ _); abstract (eauto; wrap0).
+    Defined.
+  End compileAction.
+
+
+  (** Now, create a [vcgen] version that knows about [Pat] and others, with some shameless copy-and-paste. *)
+
+  Ltac vcgen_simp := cbv beta iota zeta delta [WrapC Wrap Pat Out compileAction
+    map app imps
+    LabelMap.add Entry Blocks Postcondition VerifCond
+    Straightline_ Seq_ Diverge_ Fail_ Skip_ Assert_
+    Structured.If_ Structured.While_ Goto_ Structured.Call_ IGoto
+    setArgs Programming.Reserved Programming.Formals Programming.Precondition
+    importsMap fullImports buildLocals blocks union Nplus Nsucc length N_of_nat
+    List.fold_left ascii_lt string_lt label'_lt
+    LabelKey.compare' LabelKey.compare LabelKey.eq_dec
+    LabelMap.find
+    toCmd Programming.Seq Instr Diverge Fail Skip Assert_
+    Programming.If_ Programming.While_ Goto Programming.Call_ RvImm'
+    Assign' localsInvariant localsInvariantCont
+    regInL lvalIn immInR labelIn variableSlot string_eq ascii_eq
+    andb Bool.eqb qspecOut
+    ICall_ Structured.ICall_
+    Assert_ Structured.Assert_
+    LabelMap.Raw.find LabelMap.this LabelMap.Raw.add
+    LabelMap.empty LabelMap.Raw.empty string_dec
+    Ascii.ascii_dec string_rec string_rect sumbool_rec sumbool_rect Ascii.ascii_rec Ascii.ascii_rect
+    Bool.bool_dec bool_rec bool_rect eq_rec_r eq_rec eq_rect eq_sym
+    fst snd labl
+    Ascii.N_of_ascii Ascii.N_of_digits N.compare Nmult Pos.compare Pos.compare_cont
+    Pos.mul Pos.add LabelMap.Raw.bal
+    Int.Z_as_Int.gt_le_dec Int.Z_as_Int.ge_lt_dec LabelMap.Raw.create
+    ZArith_dec.Z_gt_le_dec Int.Z_as_Int.plus Int.Z_as_Int.max LabelMap.Raw.height
+    ZArith_dec.Z_gt_dec Int.Z_as_Int._1 BinInt.Z.add Int.Z_as_Int._0 Int.Z_as_Int._2 BinInt.Z.max
+    ZArith_dec.Zcompare_rec ZArith_dec.Z_ge_lt_dec BinInt.Z.compare ZArith_dec.Zcompare_rect
+    ZArith_dec.Z_ge_dec label'_eq label'_rec label'_rect
+    COperand1 CTest COperand2 Pos.succ
+    makeVcs
+    Note_ Note__
+    IGotoStar_ IGotoStar AssertStar_ AssertStar
+    Cond_ Cond
+  ].
+
+  Ltac vcgen := structured_auto vcgen_simp.
+
+  Definition m := bimport [["xml_lex"!"next" @ [nextS], "xml_lex"!"position" @ [positionS],
+                            "xml_lex"!"setPosition" @ [setPositionS], "xml_lex"!"tokenStart" @ [tokenStartS],
+                            "xml_lex"!"tokenLength" @ [tokenLengthS], "malloc"!"malloc" @ [mallocS],
+                            "malloc"!"free" @ [freeS], "sys"!"abort" @ [abortS], "sys"!"printInt" @ [printIntS],
+                            "xml_lex"!"init" @ [initS], "xml_lex"!"delete" @ [deleteS],
+                            "array8"!"copy" @ [copyS] ]]
+
+    bmodule "xml_prog" {{
+      {|
+        FName := "main";
+        FVars := lvars;
+        FReserved := 11;
+        FPrecondition := Precondition mainS None;
+        FBody := Programming.Seq (Assign' ((fun _ => LvMem (Indir Sp O)):lvalue') Rp)
+        (Programming.Seq (fun _ _ =>
+          Structured nil
+          (fun im mn _ =>
+            Structured.Assert_ im mn
+            (Precondition mainS (Some lvars))))
+        ("lex" <-- Call "xml_lex"!"init"("len")
+         [Al bsI, Al bsO,
+           PRE[V, R] array8 bsI (V "buf") * array8 bsO (V "obuf") * mallocHeap 0 * xmlp (V "len") R
+             * [| length bsI = wordToNat (V "len") |] * [| length bsO = wordToNat (V "olen") |]
+           POST[R'] Ex bsO', array8 bsI (V "buf") * array8 bsO' (V "obuf") * mallocHeap 0
+             * [| length bsO' = length bsO |] * [| R' <= V "olen" |]%word ];;
+         "stack" <- 0;;
+         "opos" <- 0;;
+         "overflowed" <- 0;;
+
+         Pat (fun bsO V => array8 bsO (V "obuf") * [| length bsO = wordToNat (V "olen") |]
+           * [| V "opos" <= V "olen" |]%word)%Sep
+         (fun bsO V R => Ex bsO', array8 bsO' (V "obuf") * [| length bsO' = length bsO |]
+           * [| R <= V "olen" |]%word)%Sep
+         (compilePat (Pattern pr))
+         (compileAction (Pattern pr) (Action pr));;
+
+         Call "xml_lex"!"delete"("lex")
+         [Al ls,
+           PRE[V] [| V "opos" <= V "olen" |]%word * mallocHeap 0 * sll ls (V "stack")
+           POST[R] [| R <= V "olen" |]%word * mallocHeap 0];;
+
+         [Al ls,
+           PRE[V] [| V "opos" <= V "olen" |]%word * mallocHeap 0 * sll ls (V "stack")
+           POST[R] [| R <= V "olen" |]%word * mallocHeap 0]
+         While ("stack" <> 0) {
+           "lex" <- "stack";;
+           "stack" <-* "stack"+4;;
+
+           Call "malloc"!"free"(0, "lex", 2)
+           [Al ls,
+             PRE[V] [| V "opos" <= V "olen" |]%word * mallocHeap 0 * sll ls (V "stack")
+             POST[R] [| R <= V "olen" |]%word * mallocHeap 0]
+         };;
+
+         If ("overflowed" = 1) {
+           Return 0
+         } else {
+           Return "opos"
+         }))%SP
+      |}
+    }}.
+
+
   Theorem ok : moduleOk m.
     destruct wellFormed; vcgen;
       (intros; try match goal with
                      | [ H : importsGlobal _ |- _ ] => clear H
-                   end; pre); abstract t.
+                   end; pre).
+
+    Ltac u := abstract t.
+
+    u.
+    u.
+    u.
+    u.
+    u.
+    u.
+    u.
+    u.
+    u.
+    u.
+    u.
+    u.
+    u.
+    u.
+    u.
+    u.
+    u.
+    u.
+    u.
+    u.
+    u.
+    u.
+    u.
+    u.
+    u.
+    u.
+    u.
+    u.
+    u.
+    u.
+    u.
+    u.
+    u.
+    u.
+    u.
+    u.
+    u.
+    u.
+    u.
+    u.
+    u.
+    u.
+    u.
+    u.
+    u.
+    u.
+    u.
+    u.
+    u.
+    u.
+    u.
+    u.
+    u.
+    u.
+    u.
+    u.
+    u.
   Qed.
 
 End compileProgram.
