platform/Xml.v
@@ -9,21 +9,17 @@ Infix "&" := XmlLang.Both (at level 41, right associativity) : pat_scope.
 Infix ";;" := XmlLang.Ordered : pat_scope.
 Delimit Scope pat_scope with pat.
 
-Coercion XmlOutput.Cdata : string >-> XmlOutput.xml.
-Notation "$ x" := (XmlOutput.Var (x ++ "_start")%string (x ++ "_len")%string) : out_scope.
-Definition xcons (x : XmlOutput.xml) (xs : list XmlOutput.xml) : list XmlOutput.xml := x :: xs.
-Notation "<*> tag </> x1 , .. , xN </>" := (XmlOutput.Tag tag (xcons x1 .. (xcons xN nil) ..))
+Coercion XCdata : string >-> xml.
+Notation "$ x" := (XVar x) : out_scope.
+Definition xcons (x : xml) (xs : list xml) : list xml := x :: xs.
+Notation "<*> tag </> x1 , .. , xN </>" := (XTag tag (xcons x1 .. (xcons xN nil) ..))
   (tag at level 0) : out_scope.
 Delimit Scope out_scope with out.
 
-Notation "'Match' p 'Do' o 'end'" := {| Pattern := p%pat; Output := o%out |}.
+Notation "'Write' o" := (Output o%out) (at level 0, o at level 0) : action_scope.
+Infix ";;" := Seq : action_scope.
+Delimit Scope action_scope with action.
 
-Ltac wf :=
-  repeat split; repeat constructor; simpl in *; intuition (try congruence);
-    match goal with
-      | [ H : (_, _) = (_, _) |- _ ] => injection H; clear H; intros; subst
-    end;
-    match goal with
-      | [ |- context[_ = ?s] ] => solve [ exists s; intuition ]
-    end.
+Notation "'Match' p 'Do' a 'end'" := {| Pattern := p%pat; Action := a%action |}.
 
+Ltac wf := split; [ | split ]; simpl; intuition (try (congruence || reflexivity)).
